end-to-end proof for montgomery

src/Experiments/SimplyTypedArithmetic.v
@@ -8226,12 +8226,10 @@ Module Straightline.
       | ok_scalar_cast :
           forall r s (idc : ident s  _) x,
             ok_scalar x ->
-            ok_scalar_ident idc ->
             @ok_expr type.Z (AppIdent (ident.Z.cast r) (AppIdent idc x))
       | ok_scalar_cast2 :
           forall r s (idc : ident s _) x,
             ok_scalar x ->
-            ok_scalar_ident idc ->
             @ok_expr (type.prod type.Z type.Z) (AppIdent (ident.Z.cast2 r) (AppIdent idc x))
       | ok_scalar_nocast :
           forall t x, @ok_scalar t x -> @ok_expr t x
@@ -8385,11 +8383,12 @@ Module Straightline.
         Admitted.
     End proofs.
   End expr.
-
+  
   Definition of_Expr {s d} (e : Expr (s->d)) (var : type -> Type) (x:var s) dummy_arrow: expr.expr d
     :=
       match invert_Abs (e var) with
-      | Some f => expr.of_uncurried (dummy_arrow:=dummy_arrow) (expr.depth (fun _ => unit) (fun _ => tt) (e (fun _ => unit))) (f x)
+      | Some f =>
+        expr.of_uncurried (dummy_arrow:=dummy_arrow) (expr.depth (fun _ => unit) (fun _ => tt) (e (fun _ => unit))) (f x)
       | None => expr.dummy (dummy_arrow:=dummy_arrow) d
       end.
 
@@ -8466,7 +8465,7 @@ End StraightlineTest.
 Module PreFancy.
   Import Straightline.expr.
   Section with_wordmax.
-    Context (log2wordmax : Z) (log2wordmax_pos : 1 < log2wordmax).
+    Context (log2wordmax : Z) (log2wordmax_pos : 1 < log2wordmax) (log2wordmax_even : log2wordmax mod 2 = 0).
     Let wordmax := 2 ^ log2wordmax.
     Let half_bits := log2wordmax / 2.
     Let wordmax_half_bits := 2 ^ half_bits.
@@ -8487,6 +8486,9 @@ Module PreFancy.
     Lemma wordmax_half_bits_pos : 0 < wordmax_half_bits.
     Proof. subst wordmax_half_bits half_bits. Z.zero_bounds. Qed.
 
+    Lemma half_bits_nonneg : 0 <= half_bits.
+    Proof. subst half_bits; Z.zero_bounds. Qed.
+
     Lemma half_bits_squared : (wordmax_half_bits - 1) * (wordmax_half_bits - 1) <= wordmax - 1.
     Proof.
       pose proof wordmax_half_bits_pos.
@@ -8504,8 +8506,7 @@ Module PreFancy.
     Qed.
 
     Section with_var.
-      Context {var : type -> Type} (dummy_arrow : forall s d, var (type.arrow s d))
-              (constant_to_scalar : Z -> option (@scalar var type.Z)).
+      Context {var : type -> Type} (dummy_arrow : forall s d, var (type.arrow s d)) (consts : list Z).
       Local Notation Z := (type.type_primitive type.Z).
 
       Inductive ident : type -> type -> Type :=
@@ -8526,6 +8527,20 @@ Module PreFancy.
       | addm : ident (Z * Z * Z) Z
       .
       Definition dummy t : @expr var ident t := Scalar (dummy_scalar (dummy_arrow:=dummy_arrow) t).
+
+      Definition constant_to_scalar_single (const x : BinInt.Z) : option (@scalar var Z) :=
+        if x =? (BinInt.Z.shiftr const half_bits)
+        then Some (Cast {|lower := 0; upper:=wordmax_half_bits-1|} (Shiftr half_bits (Primitive (t:=type.Z) const)))
+        else if x =? (BinInt.Z.land const (wordmax_half_bits - 1))
+             then Some (Cast {|lower := 0; upper:=wordmax_half_bits-1|} (Land (wordmax_half_bits-1) (Primitive (t:=type.Z) const)))
+             else None.
+
+      Definition constant_to_scalar (x : BinInt.Z)
+        : option (Straightline.expr.scalar Z) :=
+        fold_right (fun c res => match res with
+                                 | Some s => Some s
+                                 | None => constant_to_scalar_single c x
+                                 end) None consts.
 
       Definition invert_lower' {t} (e : @scalar var t) :
         option (@scalar var Z) :=
@@ -8669,20 +8684,6 @@ Module PreFancy.
         | LetInAppIdentZZ _ t r idc x f =>
           of_straightline_ident idc t r x (fun y => of_straightline (f y))
         end.
-
-      Definition constant_to_scalar_single (const x : BinInt.Z) : option (@scalar var Z) :=
-        if x =? (BinInt.Z.shiftr const half_bits)
-        then Some (Cast {|lower := 0; upper:=wordmax_half_bits-1|} (Shiftr half_bits (Primitive (t:=type.Z) const)))
-        else if x =? (BinInt.Z.land const (wordmax_half_bits - 1))
-             then Some (Cast {|lower := 0; upper:=wordmax_half_bits-1|} (Land (wordmax_half_bits-1) (Primitive (t:=type.Z) const)))
-             else None.
-
-      Definition constant_to_scalar_gen (consts : list BinInt.Z) (x : BinInt.Z)
-        : option (Straightline.expr.scalar Z) :=
-        fold_right (fun c res => match res with
-                                 | Some s => Some s
-                                 | None => constant_to_scalar_single c x
-                                 end) None consts.
     End with_var.
 
     Section interp.
@@ -8719,8 +8720,8 @@ Module PreFancy.
     End interp.
 
     Section proofs.
-      Context (dummy_arrow : forall s d, type.interp (s -> d)%ctype)
-              (constant_to_scalar : Z -> option (@scalar type.interp type.Z)).
+      Context (dummy_arrow : forall s d, type.interp (s -> d)%ctype) (consts : list Z)
+              (consts_ok : forall x, In x consts -> 0 <= x <= wordmax - 1).
 
       Local Notation word_range := (r[0~>wordmax-1])%zrange.
       Local Notation half_word_range := (r[0~>wordmax_half_bits-1])%zrange.
@@ -8799,7 +8800,22 @@ Module PreFancy.
       | sc_ok_prim : forall p x, ok_scalar (@Primitive _ p x)
       .
 
-      Print ident.
+      Inductive is_halved : scalar type.Z -> Prop :=
+      | is_halved_lower :
+          forall x : scalar type.Z,
+            in_word_range (get_range x) ->
+            is_halved (Cast half_word_range (Land (wordmax_half_bits - 1) x))
+      | is_halved_upper :
+          forall x : scalar type.Z,
+            in_word_range (get_range x) ->
+            is_halved (Cast half_word_range (Shiftr half_bits x))
+      | is_halved_constant :
+          forall y z,
+            constant_to_scalar consts z = Some y ->
+            is_halved y ->
+            is_halved (Primitive (t:=type.Z) z)
+      .
+
       Inductive ok_ident : forall s d, scalar s -> range_type d -> ident.ident s d -> Prop :=
       | ok_add :
           forall x : scalar (type.prod type.Z type.Z),
@@ -8835,14 +8851,16 @@ Module PreFancy.
             0 <= n < wordmax ->
             ok_ident type.Z type.Z x (ZRange.map (fun y => Z.land y n) (get_range x)) (ident.Z.land n)*)
       | ok_shiftr :
-          forall (x : scalar type.Z) n,
+          forall (x : scalar type.Z) n r,
             in_word_range (get_range x) ->
             0 <= n <= log2wordmax ->
-            ok_ident type.Z type.Z x (ZRange.map (fun y => Z.shiftr y n) (get_range x)) (ident.Z.shiftr n)
+            r = ZRange.map (fun y => Z.shiftr y n) (get_range x) ->
+            ok_ident type.Z type.Z x r (ident.Z.shiftr n)
       | ok_shiftl :
           forall (x : scalar type.Z) n,
             in_word_range (get_range x) ->
-            0 <= n < log2wordmax - Z.log2_up (upper (get_range x)) ->
+            0 <= n ->
+            upper (get_range x) * 2 ^ n <= wordmax - 1 ->
             ok_ident type.Z type.Z x word_range (ident.Z.shiftl n)
       | ok_rshi :
           forall (x : scalar (type.prod type.Z type.Z)) n,
@@ -8857,7 +8875,7 @@ Module PreFancy.
             in_word_range (get_range z) ->
             ok_ident _ 
                      type.Z
-                     (Pair (Pair (Snd x) y) z)
+                     (Pair (Pair (Cast flag_range (Snd x)) y) z)
                      word_range
                      ident.Z.zselect
       | ok_selm :
@@ -8891,6 +8909,16 @@ Module PreFancy.
                      x 
                      word_range
                      ident.Z.add_modulo
+      | ok_mul :
+          forall x y : scalar type.Z,
+            is_halved x ->
+            is_halved y ->
+            ok_ident (type.prod type.Z type.Z)
+                     type.Z
+                     (Pair x y)
+                     word_range
+                     ident.Z.mul
+                     (*
       | ok_mulll :
           forall x y : scalar type.Z,
             in_word_range (get_range x) ->
@@ -8935,6 +8963,7 @@ Module PreFancy.
                         (Cast half_word_range (Shiftr half_bits y)))
                      word_range
                      ident.Z.mul
+*)
       .
 
       Inductive ok_expr : forall {t}, @expr type.interp ident.ident t -> Prop :=
@@ -9061,7 +9090,7 @@ Module PreFancy.
       Qed.
 
       Lemma has_word_range_shiftl n r x :
-        0 <= n < log2wordmax - Z.log2_up (upper r) ->
+        0 <= n -> upper r * 2 ^ n <= wordmax - 1 ->
         @has_range type.Z r x ->
         in_word_range r ->
         @has_range type.Z word_range (x << n).
@@ -9073,18 +9102,7 @@ Module PreFancy.
         apply andb_true_iff; split; apply Z.leb_le;
           [ apply Z.shiftl_nonneg; solve [auto using in_word_range_nonneg] | ].
         rewrite Z.shiftl_mul_pow2 by omega.
-        destruct (dec (upper r = 0));
-          [ match goal with H : _ = 0 |- _ => rewrite H end; pose proof wordmax_gt_2; lia | ].
-        match goal with |- ?a * ?b <= _ =>
-                        transitivity (2 ^ (Z.log2_up a) * b) end.
-        { apply Z.mul_le_mono_nonneg_r; auto with zarith; [ ].
-          apply Z.log2_log2_up_spec.
-          apply Z.le_neq; eauto using in_word_range_upper_nonneg with has_range. }
-        { rewrite <-Z.pow_add_r by auto with zarith.
-          assert (2 ^ (Z.log2_up (upper r) + n) < 2 ^ log2wordmax)
-            by (apply Z.pow_lt_mono_r; omega).
-          replace wordmax with (2 ^ log2wordmax) by reflexivity.
-          omega. }
+        auto.
       Qed.
 
       Lemma has_word_range_rshi n x y :
@@ -9098,12 +9116,12 @@ Module PreFancy.
       Qed.
 
       Lemma in_word_range_spec r :
-        0 <= lower r -> upper r <= wordmax - 1 ->
-        in_word_range r.
+        (0 <= lower r /\ upper r <= wordmax - 1)
+        <-> in_word_range r.
       Proof.
         intros; cbv [in_word_range is_tighter_than_bool].
-        apply andb_true_iff.
-        split; apply Z.leb_le; cbn [upper lower]; omega.
+        rewrite andb_true_iff.
+        intuition; apply Z.leb_le; cbn [upper lower]; try omega.
       Qed.
 
       Ltac destruct_scalar :=
@@ -9119,6 +9137,150 @@ Module PreFancy.
           end
         end.
 
+      Ltac extract_ok_scalar' level x :=
+        match goal with
+        | H : ok_scalar (Pair (Pair (?f (?g x)) _) _) |- _ =>
+          match (eval compute in (4 <=? level)) with
+          | true => invert H; extract_ok_scalar' 3 x
+          | _ => fail
+          end
+        | H : ok_scalar (Pair (?f (?g x)) _) |- _ =>
+          match (eval compute in (3 <=? level)) with
+          | true => invert H; extract_ok_scalar' 2 x
+          | _ => fail
+          end
+        | H : ok_scalar (Pair _ (?f (?g x))) |- _ =>
+          match (eval compute in (3 <=? level)) with
+          | true => invert H; extract_ok_scalar' 2 x
+          | _ => fail
+          end
+        | H : ok_scalar (?f (?g x)) |- _ =>
+          match (eval compute in (2 <=? level)) with
+          | true => invert H; extract_ok_scalar' 1 x
+          | _ => fail
+          end
+        | H : ok_scalar (?g x) |- _ => invert H
+        | H : ok_scalar (Pair x _) |- _ => invert H
+        | H : ok_scalar (Pair _ x) |- _ => invert H
+        end.
+
+      Ltac extract_ok_scalar :=
+        match goal with |- ok_scalar ?x => extract_ok_scalar' 4 x; assumption end.
+
+      Lemma has_half_word_range_shiftr r x :
+        in_word_range r ->
+        @has_range type.Z r x ->
+        @has_range type.Z half_word_range (x >> half_bits).
+      Proof.
+        cbv [in_word_range is_tighter_than_bool].
+        rewrite andb_true_iff.
+        cbn [has_range upper lower]; intros; intuition; Z.ltb_to_lt.
+        { apply Z.shiftr_nonneg. omega. }
+        { pose proof half_bits_nonneg.
+          pose proof half_bits_squared.
+          assert (x >> half_bits < wordmax_half_bits); [|omega].
+          rewrite Z.shiftr_div_pow2 by auto.
+          apply Z.div_lt_upper_bound; Z.zero_bounds.
+          subst wordmax_half_bits half_bits.
+          rewrite <-Z.pow_add_r by omega.
+          rewrite Z.add_diag, Z.mul_div_eq, log2wordmax_even by omega.
+          autorewrite with zsimplify_fast. subst wordmax. omega. }
+      Qed.
+
+      Lemma has_half_word_range_land r x :
+        in_word_range r ->
+        @has_range type.Z r x ->
+        @has_range type.Z half_word_range (x &' (wordmax_half_bits - 1)).
+      Proof.
+        pose proof wordmax_half_bits_pos.
+        cbv [in_word_range is_tighter_than_bool].
+        rewrite andb_true_iff.
+        cbn [has_range upper lower]; intros; intuition; Z.ltb_to_lt.
+        { apply Z.land_nonneg; omega. }
+        { apply Z.land_upper_bound_r; omega. }
+      Qed.
+
+      Section constant_to_scalar.
+        Lemma constant_to_scalar_single_correct s x z :
+            0 <= x <= wordmax - 1 ->
+            constant_to_scalar_single x z = Some s -> interp_scalar s = z.
+        Proof.
+          cbv [constant_to_scalar_single].
+          break_match; try discriminate; intros; Z.ltb_to_lt; subst;
+            try match goal with H : Some _ = Some _ |- _ => inversion H; subst end;
+            cbn [interp_scalar]; apply interp_cast_noop.
+          { apply has_half_word_range_shiftr with (r:=r[x~>x]%zrange);
+            cbv [in_word_range is_tighter_than_bool upper lower has_range]; try omega.
+            apply andb_true_iff; split; apply Z.leb_le; omega. }
+          { apply has_half_word_range_land with (r:=r[x~>x]%zrange);
+            cbv [in_word_range is_tighter_than_bool upper lower has_range]; try omega.
+            apply andb_true_iff; split; apply Z.leb_le; omega. }
+        Qed.
+
+        Lemma constant_to_scalar_correct s z :
+          constant_to_scalar consts z = Some s -> interp_scalar s = z.
+        Proof.
+          cbv [constant_to_scalar].
+          apply fold_right_invariant; try discriminate.
+          intros until 2; break_match; eauto using constant_to_scalar_single_correct.
+        Qed.
+
+        Lemma constant_to_scalar_single_cases x y z :
+          @constant_to_scalar_single type.interp x z = Some y -> 
+          (y = Cast half_word_range (Land (wordmax_half_bits - 1) (Primitive (t:=type.Z) x)))
+          \/ (y = Cast half_word_range (Shiftr half_bits (Primitive (t:=type.Z) x))).
+        Proof.
+          cbv [constant_to_scalar_single].
+          break_match; try discriminate; intros; Z.ltb_to_lt; subst;
+            try match goal with H : Some _ = Some _ |- _ => inversion H; subst end;
+            tauto.
+        Qed.
+
+        Lemma constant_to_scalar_cases y z :
+          @constant_to_scalar type.interp consts z = Some y ->
+          (exists x,
+              @has_range type.Z word_range x
+              /\ y = Cast half_word_range (Land (wordmax_half_bits - 1) (Primitive x)))
+          \/ (exists x,
+                 @has_range type.Z word_range x
+                 /\ y = Cast half_word_range (Shiftr half_bits (Primitive x))).
+        Proof.
+          cbv [constant_to_scalar].
+          apply fold_right_invariant; try discriminate.
+          intros until 2; break_match; eauto; intros.
+          match goal with H : constant_to_scalar_single _ _ = _ |- _ =>
+                          destruct (constant_to_scalar_single_cases _ _ _ H); subst end.
+          { left; eexists; split; eauto.
+            apply consts_ok; auto. }
+          { right; eexists; split; eauto.
+            apply consts_ok; auto. }
+        Qed.
+
+        Lemma ok_scalar_constant_to_scalar y z : constant_to_scalar consts z = Some y -> ok_scalar y.
+        Proof.
+          pose proof wordmax_half_bits_pos. pose proof half_bits_nonneg.
+          let H := fresh in
+          intro H; apply constant_to_scalar_cases in H; destruct H as [ [? ?] | [? ?] ]; intuition; subst;
+            cbn [has_range lower upper] in *; repeat constructor; cbn [lower get_range]; try apply Z.leb_refl; try omega.
+          assert (in_word_range r[x~>x]) by (apply in_word_range_spec; cbn [lower upper]; omega).
+          pose proof (has_half_word_range_shiftr r[x~>x] x ltac:(assumption) ltac:(cbv [has_range lower upper]; omega)).
+          cbn [has_range ZRange.map is_tighter_than_bool lower upper] in *.
+          apply andb_true_iff; cbn [lower upper]; split; apply Z.leb_le; omega.
+        Qed.
+      End constant_to_scalar.
+      Hint Resolve ok_scalar_constant_to_scalar.
+
+      Lemma is_halved_has_range x :
+        ok_scalar x ->
+        is_halved x ->
+        @has_range type.Z half_word_range (interp_scalar x).
+      Proof.
+        intro; pose proof (has_range_interp_scalar x ltac:(assumption)).
+        induction 1; cbn [interp_scalar] in *; intros; try assumption; [ ].
+        rewrite <-(constant_to_scalar_correct y z) by assumption.
+        eauto using has_range_interp_scalar.
+      Qed.
+
       Lemma ident_interp_has_range s d x r idc:
         ok_scalar x ->
         ok_ident s d x r idc ->
@@ -9131,6 +9293,7 @@ Module PreFancy.
           repeat match goal with
                  | H : _ && _ = true |- _ => rewrite andb_true_iff in H; destruct H; Z.ltb_to_lt
                  |  H : _ /\ _ |- _ => destruct H
+                 | H : is_halved _ |- _ => apply is_halved_has_range in H; [ | extract_ok_scalar ]
                  | _ => progress subst
                  | _ => progress (cbv [in_word_range in_flag_range is_tighter_than_bool] in * )
                  | _ => progress (cbn [interp_scalar get_range has_range upper lower fst snd] in * )
@@ -9151,7 +9314,8 @@ Module PreFancy.
           rewrite Z.div_sub_small by omega.
           split; break_match; lia. }
         { apply has_range_shiftr; cbn [has_range]; omega. }
-        { eapply has_word_range_shiftl; eauto using in_word_range_spec with has_range omega. }
+        { eapply has_word_range_shiftl; eauto  with has_range omega.
+          apply in_word_range_spec ; omega. }
         { apply has_word_range_rshi; omega. }
         { rewrite Z.zselect_correct. break_match; omega. }
         { cbn [interp_scalar fst snd get_range] in *.
@@ -9160,39 +9324,9 @@ Module PreFancy.
           rewrite Z.zselect_correct. break_match; omega. }
         { rewrite Z.add_modulo_correct.
           break_match; Z.ltb_to_lt; omega. }
-        { cbn [interp_scalar fst snd get_range upper lower] in *.
-          pose proof half_bits_squared. nia. }
-        { cbn [interp_scalar fst snd get_range upper lower] in *.
-          pose proof half_bits_squared. nia. }
-        { cbn [interp_scalar fst snd get_range upper lower] in *.
-          pose proof half_bits_squared. nia. }
-        { cbn [interp_scalar fst snd get_range upper lower] in *.
+        { cbn [interp_scalar has_range fst snd get_range upper lower] in *.
           pose proof half_bits_squared. nia. }
       Qed.
-
-      Ltac extract_ok_scalar' level x :=
-        match goal with
-        | H : ok_scalar (Pair (Pair (?f (?g x)) _) _) |- _ =>
-          match (eval compute in (4 <=? level)) with
-          | true => invert H; extract_ok_scalar' 3 x
-          | _ => fail
-          end
-        | H : ok_scalar (Pair (?f (?g x)) _) |- _ =>
-          match (eval compute in (3 <=? level)) with
-          | true => invert H; extract_ok_scalar' 2 x
-          | _ => fail
-          end
-        | H : ok_scalar (?f (?g x)) |- _ =>
-          match (eval compute in (2 <=? level)) with
-          | true => invert H; extract_ok_scalar' 1 x
-          | _ => fail
-          end
-        | H : ok_scalar (?g x) |- _ => invert H
-        end.
-      
-
-      Ltac extract_ok_scalar :=
-        match goal with |- ok_scalar ?x => extract_ok_scalar' 4 x; assumption end.
 
       Lemma has_flag_range_cc_m r x :
         @has_range type.Z r x ->
@@ -9239,16 +9373,76 @@ Module PreFancy.
                | _ => rewrite interp_cast_noop by assumption
                end.
 
+      Lemma is_halved_cases x :
+        is_halved x ->
+        ok_scalar x ->
+        (exists y,
+            invert_lower consts x = Some y
+            /\ invert_upper consts x = None
+            /\ interp_scalar y &' (wordmax_half_bits - 1) = interp_scalar x)
+        \/ (exists y,
+               invert_lower consts x = None
+               /\ invert_upper consts x = Some y
+               /\ interp_scalar y >> half_bits = interp_scalar x).
+      Proof.
+        induction 1; intros; cbn; rewrite ?Z.eqb_refl; cbn.
+        { left. eexists; repeat split; auto.
+          rewrite interp_cast_noop; [ reflexivity | ].
+          apply has_half_word_range_land with (r:=get_range x); auto.
+          apply has_range_interp_scalar; extract_ok_scalar. }
+        { right. eexists; repeat split; auto.
+          rewrite interp_cast_noop; [ reflexivity | ].
+          apply has_half_word_range_shiftr with (r:=get_range x); auto.
+          apply has_range_interp_scalar; extract_ok_scalar. }
+        { match goal with H : constant_to_scalar _ _ = Some _ |- _ =>
+                          rewrite H;
+                            let P := fresh in
+                            destruct (constant_to_scalar_cases _ _ H) as [ [? [? ?] ] | [? [? ?] ] ];
+                              subst; cbn; rewrite ?Z.eqb_refl; cbn
+          end.
+          { left; eexists; repeat split; auto.
+            erewrite <-constant_to_scalar_correct by eassumption.
+            subst. cbn.
+            rewrite interp_cast_noop; [ reflexivity | ].
+            eapply has_half_word_range_land with (r:=word_range); auto.
+            cbv [in_word_range is_tighter_than_bool].
+            rewrite !Z.leb_refl; reflexivity. }
+          { right; eexists; repeat split; auto.
+            erewrite <-constant_to_scalar_correct by eassumption.
+            subst. cbn.
+            rewrite interp_cast_noop; [ reflexivity | ].
+            eapply has_half_word_range_shiftr with (r:=word_range); auto.
+            cbv [in_word_range is_tighter_than_bool].
+            rewrite !Z.leb_refl; reflexivity. } }
+      Qed.
+
+      Lemma of_straightline_ident_mul_correct t x y g :
+        is_halved x ->
+        is_halved y ->
+        ok_scalar (Pair x y) ->
+        @has_range type.Z word_range (ident.interp ident.Z.mul (interp_scalar (Pair x y))) ->
+        interp (of_straightline_ident dummy_arrow consts ident.Z.mul t word_range (Pair x y) g) =
+        interp (g (ident.interp ident.Z.mul (interp_scalar (Pair x y)))).
+      Proof.
+        intros Hx Hy Hok ?; invert Hok; cbn [interp_scalar of_straightline_ident].
+        destruct (is_halved_cases x Hx ltac:(assumption)) as [ [? [Pxlow [Pxhigh Pxi] ] ] | [? [Pxlow [Pxhigh Pxi] ] ] ];
+          rewrite ?Pxlow, ?Pxhigh;
+          destruct (is_halved_cases y Hy ltac:(assumption)) as [ [? [Pylow [Pyhigh Pyi] ] ] | [? [Pylow [Pyhigh Pyi] ] ] ];
+          rewrite ?Pylow, ?Pyhigh;
+          cbn; rewrite Pxi, Pyi; rewrite interp_cast_noop by auto; reflexivity.
+      Qed.
+
       Lemma of_straightline_ident_correct s d t x r (idc : ident.ident s d) g :
         ok_ident s d x r idc ->
         ok_scalar x ->
-        interp (of_straightline_ident dummy_arrow constant_to_scalar idc t r x g) =
+        interp (of_straightline_ident dummy_arrow consts idc t r x g) =
         interp (g (ident.interp idc (interp_scalar x))).
       Proof.
         intros.
         pose proof wordmax_half_bits_pos.
         pose proof (ident_interp_has_range _ _ x r idc ltac:(assumption) ltac:(assumption)).
-        induction H; cbn [of_straightline_ident ident.interp ident.gen_interp invert_selm invert_sell invert_upper invert_lower invert_upper' invert_lower'] in *; intros;
+        induction H; try solve [auto using of_straightline_ident_mul_correct];
+          cbn [of_straightline_ident ident.interp ident.gen_interp invert_selm invert_sell] in *; intros;
           rewrite ?Z.eqb_refl; cbn [interp interp_ident andb]; try destruct_scalar;
             repeat match goal with
                    | _ => progress (cbn [fst snd interp_scalar] in * )
@@ -9261,16 +9455,12 @@ Module PreFancy.
                    | _ => rewrite interp_cast_noop by assumption
                    | _ => rewrite interp_cast2_noop by assumption
                    | _ => reflexivity
-                   end; [ | | | ]; (* leftover cases are the 4 kinds of multiplication *)
-              match goal with
-              | H1 : in_word_range (get_range ?x), H2 : in_word_range (get_range ?y) |- _ =>
-                extract_ok_scalar' 4 x; extract_ok_scalar' 4 y
-              end; rewrite_cast_noop_in_mul; reflexivity.
+                   end.
       Qed.
 
       Lemma of_straightline_correct {t} (e : expr t) :
         ok_expr e ->
-        interp (of_straightline dummy_arrow constant_to_scalar e) = Straightline.expr.interp (interp_ident:=@ident.interp) e.
+        interp (of_straightline dummy_arrow consts e) = Straightline.expr.interp (interp_ident:=@ident.interp) e.
       Proof.
         induction 1; cbn [of_straightline]; intros;
           repeat match goal with
@@ -9287,16 +9477,19 @@ Module PreFancy.
 
   Definition of_Expr {s d} (log2wordmax : Z) (consts : list Z) (e : Expr (s -> d))
              (var : type -> Type) (x : var s) dummy_arrow : @Straightline.expr.expr var ident d :=
-    @of_straightline log2wordmax var dummy_arrow (@constant_to_scalar_gen log2wordmax var consts) _ (Straightline.of_Expr e var x dummy_arrow).
+    @of_straightline log2wordmax var dummy_arrow consts _ (Straightline.of_Expr e var x dummy_arrow).
 
   Lemma of_Expr_correct {s d} (log2wordmax : Z) (consts : list Z) (e : Expr (s -> d))
         (e' : (type.interp s -> Uncurried.expr.expr d))
         (x : type.interp s) dummy_arrow :
     e type.interp = Abs e' ->
     1 < log2wordmax ->
+    log2wordmax mod 2 = 0 ->
     Straightline.expr.ok_expr (e' x) ->
-    ok_expr log2wordmax (of_uncurried (dummy_arrow:=dummy_arrow) (depth (fun _ : type => unit) (fun _ : type => tt) (e (fun _ : type => unit))) (e' x)) ->
-    (depth type.interp (@DefaultValue.type.default) (e' x) <= depth (fun _ : type => unit) (fun _ : type => tt) (e (fun _ : type => unit)))%nat ->
+    (forall x0 : Z, In x0 consts -> 0 <= x0 <= 2 ^ log2wordmax - 1) ->
+    ok_expr log2wordmax consts
+            (of_uncurried (dummy_arrow:=dummy_arrow) (depth (fun _ : type => unit) (fun _ : type => tt) (e _)) (e' x)) ->
+    (depth type.interp (@DefaultValue.type.default) (e' x) <= depth (fun _ : type => unit) (fun _ : type => tt) (e _))%nat ->
     interp log2wordmax (of_Expr log2wordmax consts e type.interp x dummy_arrow) = @Uncurried.expr.interp _ (@ident.interp) _ (e type.interp) x.
   Proof.
     intro He'; intros; cbv [of_Expr Straightline.of_Expr].
@@ -10542,15 +10735,113 @@ Ltac solve_rmontred_nocache := solve_rop_nocache MontgomeryReduction.rmontred_co
 
 Module Montgomery256.
 
-  Definition N := (2^256-2^224+2^192+2^96-1).
+  Definition N := Eval lazy in (2^256-2^224+2^192+2^96-1).
   Definition N':= (115792089210356248768974548684794254293921932838497980611635986753331132366849).
-  Definition R := (2^256).
+  Definition R := Eval lazy in (2^256).
   Definition machine_wordsize := 256.
 
   Derive montred256
          SuchThat (MontgomeryReduction.rmontred_correctT N R N' machine_wordsize montred256)
          As montred256_correct.
   Proof. Time solve_rmontred machine_wordsize. Time Qed.
+
+
+  Lemma montred'_correct_specialized R' (R'_correct : Z.equiv_modulo N (R * R') 1) :
+    forall (lo hi : Z),
+      0 <= lo < R -> 0 <= hi < R -> 0 <= lo + R * hi < R * N ->
+      MontgomeryReduction.montred' N R N' (Z.log2 R) 2 2 (lo, hi) = ((lo + R * hi) * R') mod N.
+  Proof.
+    intros.
+    apply MontgomeryReduction.montred'_correct with (T:=lo + R * hi) (R':=R');
+      try match goal with
+            | |- context[R'] => assumption
+            | |- context [lo] =>
+              try assumption; progress autorewrite with zsimplify cancel_pair; reflexivity
+          end; lazy; try split; congruence.
+  Qed.
+
+  (* Note: If this is not factored out, then for some reason Qed takes forever in montred256_correct_full. *)
+  Lemma montred256_correct_proj2 :
+    forall xy : type.interp (type.prod type.Z type.Z),
+      ZRange.type.option.is_bounded_by
+        (t:=type.prod type.Z type.Z)
+        (Some r[0 ~> 2 ^ machine_wordsize - 1]%zrange, Some r[0 ~> 2 ^ machine_wordsize - 1]%zrange)
+        xy = true ->
+       expr.Interp (@ident.interp) montred256 xy = MontgomeryReduction.montred' N R N' (Z.log2 R) 2 2 xy.
+  Proof. intros; destruct (montred256_correct xy); assumption. Qed.
+
+  Lemma montred256_correct_full  R' (R'_correct : Z.equiv_modulo N (R * R') 1) :
+    forall (lo hi : Z),
+      0 <= lo < R -> 0 <= hi < R -> 0 <= lo + R * hi < R * N ->
+      expr.interp (@ident.interp) (montred256 type.interp) (lo, hi) = ((lo + R * hi) * R') mod N.
+  Proof.
+    intros.
+    rewrite <-montred'_correct_specialized by assumption.
+    rewrite <-montred256_correct_proj2.
+    { cbv [expr.Interp type.uncurried_domain type.uncurry type.final_codomain].
+      reflexivity. }
+    { cbn. rewrite !andb_true_iff. cbv [R N] in *.
+      repeat split; apply Z.leb_le; omega. }
+  Qed.
+
+  (* TODO : maybe move these ok_expr tactics somewhere else *)
+  Ltac ok_expr_step' :=
+    match goal with
+    | _ => assumption
+    | |- context [PreFancy.ok_ident] => constructor
+    | |- context [PreFancy.ok_scalar] => constructor; try omega
+    | |- context [PreFancy.is_halved] => eapply PreFancy.is_halved_constant; [lazy; reflexivity | ]
+    | |- context [PreFancy.is_halved] => constructor
+    | |- context [PreFancy.in_word_range] => lazy; reflexivity
+    | |- context [PreFancy.in_flag_range] => lazy; reflexivity
+    | |- context [PreFancy.get_range] =>
+      cbn [PreFancy.get_range lower upper fst snd ZRange.map]
+    | x : type.interp (type.prod _ _) |- _ => destruct x
+    | |- (_ <=? _)%zrange = true =>
+      match goal with
+      | |- context [PreFancy.get_range_var] =>
+        cbv [is_tighter_than_bool PreFancy.has_range fst snd upper lower R N] in *; cbn;
+        apply andb_true_iff; split; apply Z.leb_le
+      | _ => lazy
+      end; omega || reflexivity
+    | |- @eq zrange _ _ => lazy; reflexivity
+    | |- _ <= _ => cbv [machine_wordsize]; omega
+    | |- _ <= _ <= _ => cbv [machine_wordsize]; omega
+    end; intros.
+
+  (* TODO : maybe move these ok_expr tactics somewhere else *)
+  Ltac ok_expr_step :=
+    match goal with
+    | |- context [PreFancy.ok_expr] => constructor; cbn [fst snd]; repeat ok_expr_step'
+    end; intros; cbn [Nat.max].
+
+  Definition montred256_prefancy' := PreFancy.of_Expr machine_wordsize [N;N'] montred256.
+
+  Derive montred256_prefancy
+         SuchThat (montred256_prefancy = montred256_prefancy' type.interp)
+         As montred256_prefancy_eq.
+  Proof. lazy - [type.interp]; reflexivity. Qed.
+
+  Lemma montred256_prefancy_correct R' (R'_correct : Z.equiv_modulo N (R * R') 1) :
+    forall (lo hi : Z) dummy_arrow,
+      0 <= lo < R -> 0 <= hi < R -> 0 <= lo + R * hi < R * N ->
+      @PreFancy.interp machine_wordsize type.Z (montred256_prefancy (lo,hi) dummy_arrow) = ((lo + R * hi) * R') mod N.
+  Proof.
+    intros. rewrite montred256_prefancy_eq; cbv [montred256_prefancy'].
+    erewrite PreFancy.of_Expr_correct.
+    { apply montred256_correct_full; assumption. }
+    { reflexivity. } 
+    { lazy; reflexivity. }
+    { lazy; reflexivity. }
+    { repeat constructor. }
+    { cbv [In N N']; intros; intuition; subst; cbv; congruence. }
+    { assert (340282366920938463463374607431768211455 * 2 ^ 128 <= 2 ^ machine_wordsize - 1) as shiftl_128_ok by (lazy; congruence).
+      repeat (ok_expr_step; [ ]).
+      ok_expr_step.
+      lazy; congruence.
+      constructor. }
+    { lazy. omega. }
+   Qed.
 
   Import PrintingNotations.
   Set Printing Width 10000.
@@ -10585,8 +10876,7 @@ montred256 = fun var : type -> Type => (λ x : var (type.type_primitive type.Z *
      : Expr (type.uncurry (type.type_primitive type.Z * type.type_primitive type.Z -> type.type_primitive type.Z))
 *)
 
-  Definition montred256_prefancy :=
-    Eval lazy in (PreFancy.of_Expr machine_wordsize [N;N'] montred256).
+
   Import PreFancy.
   Import PreFancy.Notations.
   Local Notation "'RegMod'" := (Straightline.expr.Primitive (t:=type.Z) 115792089210356248762697446949407573530086143415290314195533631308867097853951).
